\begin{eqnarray*}
	\sum_{k=1}^n k &=& \frac12 (n^2 + n) = \frac12 n(n+1) \\
	\sum_{k=1}^n k^2 &=& \frac16 (2n^3+3n^2+n) = \frac16 n(n+1)(2n+1) \\
	\sum_{k=1}^n k^3 &=& \frac14 (n^4+2n^3+n^2) = \frac4 n^2(n+1)^2 \\
	\sum_{k=1}^n k^4 &=& \frac1{30} (6n^5+15n^4+10n^3-n) = \frac1{30} n(n+1)(2n+1)(3n^2+3n+1) \\
	\sum_{k=1}^n k^5 &=& \frac1{12} (2n^6+6n^5+5n^4-n^2) = \frac1{12} n^2(n+1)^2(2n^2+2n-1) \\
	\sum_{k=1}^n k^6 &=& \frac1{42} (6n^7+21n^6+21n^5-7n^3+n) = \frac1{42} n(n+1)(2n+1)(3n^4+6n^3-3n+1)
\end{eqnarray*}
